Update rule

src/ecPrinting.ml
@@ -2978,15 +2978,17 @@ let pp_hoareF (ppe : PPEnv.t) ?prpo fmt hf =
 let pp_hoareS (ppe : PPEnv.t) ?prpo fmt hs =
   let ppef = PPEnv.push_mem ppe ~active:true hs.hs_m in
   let ppnode = collect2_s ppef hs.hs_s.s_node [] in
-  let ppnode = c_ppnode ~width:ppe.PPEnv.ppe_width ppef ppnode
-  in
-    Format.fprintf fmt "Context : %a@\n%!" (pp_memtype ppe) (snd hs.hs_m);
-    Format.fprintf fmt "@\n%!";
-    Format.fprintf fmt "%a%!" (pp_pre ppef ?prpo) hs.hs_pr;
-    Format.fprintf fmt "@\n%!";
-    Format.fprintf fmt "%a" (pp_node `Left) ppnode;
-    Format.fprintf fmt "@\n%!";
-    Format.fprintf fmt "%a%!" (pp_post ppef ?prpo) hs.hs_po
+  let ppnode = c_ppnode ~width:ppe.PPEnv.ppe_width ppef ppnode in
+
+  Format.fprintf fmt "Context : %a@\n%!" (pp_memtype ppe) (snd hs.hs_m);
+  Format.fprintf fmt "@\n%!";
+  Format.fprintf fmt "%a%!" (pp_pre ppef ?prpo) hs.hs_pr;
+  Format.fprintf fmt "@\n%!";
+  Format.fprintf fmt "%a" (pp_node `Left) ppnode;
+  Format.fprintf fmt "@\n%!";
+  Format.fprintf fmt "%a%!" (pp_post ppef ?prpo) hs.hs_po;
+  Format.fprintf fmt "@\n%!";
+  Format.fprintf fmt "%a%!" (pp_poe ppef ?prpo) hs.hs_poe
 
 (* -------------------------------------------------------------------- *)
 let pp_eHoareF (ppe : PPEnv.t) ?prpo fmt hf =
